Lgen.v
@@ -1,0 +1,208 @@
+Set Implicit Arguments.
+
+Require Import List Program.
+
+Require Import LibTactics Omega.
+Require Import TyOrder Subst Ty Arith_base.
+
+Include SUBST.
+Include TYORDER.
+
+Inductive ground_ty : Type :=
+  | skolem : nat -> ground_ty
+  | con : nat -> ground_ty
+  | app : ground_ty -> ground_ty -> ground_ty.
+
+Definition eq_ground_ty_dec : forall (t t' : ground_ty) , {t = t'} + {t <> t'}.
+   pose eq_nat_dec.
+   decide equality.
+Defined.
+
+Inductive leq_ground : ground_ty -> ground_ty -> Prop :=
+  | leq_skolem : forall n t, leq_ground (skolem n) t
+  | leq_con : forall n, leq_ground (con n) (con n)
+  | leq_app : forall l l' r r', leq_ground l l' -> leq_ground r r' -> leq_ground (app l r) (app l' r').
+
+Hint Constructors leq_ground.
+
+Obligation Tactic := intuition ; program_simpl ; 
+                       repeat 
+                         (match goal with
+                            | [H : leq_ground _ _ |- _] => inverts* H
+                          end).
+
+Program Fixpoint leq_ground_dec (t t' : ground_ty) : {leq_ground t t'} + {~ leq_ground t t'} :=
+  match t,t' with
+    | skolem n, t' => left _
+    | con n, con n'=>
+        match eq_nat_dec n n' with
+           | left _ => left _
+           | right _ => right _
+        end
+    | con _, skolem _ =>
+        right _ 
+    | con _, app _ _ => 
+        right _ 
+    | app l r, app l' r' =>
+        match leq_ground_dec l l', leq_ground_dec r r' with
+          | left _, left _ =>  left _
+          | left _, right _ => right _
+          | right _, left _ => right _
+          | right _, right _ => right _
+        end
+    | app _ _, con _ =>
+        right _
+    | app _ _, skolem _ => 
+        right _
+  end.
+
+Fixpoint skolemize (t : ty) : ground_ty :=
+  match t with
+    | tvar n => skolem n
+    | tcon n => con n
+    | tapp l r => app (skolemize l) (skolemize r)
+  end.
+
+Fixpoint unskolemize (t : ground_ty) : ty :=
+  match t with
+    | skolem n => tvar n
+    | con n => tcon n
+    | app l r => tapp (unskolemize l) (unskolemize r)
+  end.
+
+Fixpoint skolem_vars (t : ground_ty) : list nat :=
+  match t with
+    | skolem n => n :: nil
+    | con n    => nil
+    | app l r  => skolem_vars l ++ skolem_vars r 
+  end.
+
+Obligation Tactic := program_simpl ; intuition ; 
+              (repeat (match goal with
+                       | [H : _ \/ _ |- _] => destruct H ; subst
+                       | [H : context[In _ _ -> _], 
+                          H1 : In _ _ |- _] => apply H in H1 ; try omega
+                       end)).
+
+Program Fixpoint max_list (l : list nat) : {n | forall n', In n' l -> n > n'} :=
+  match l with
+    | nil => 0
+    | x :: l' =>
+        match max_list l' with
+          | x' => match le_gt_dec x x' with
+                    | left _  => S x'
+                    | right _ => S x
+                  end
+        end
+  end.
+
+Definition gen_list := list (ground_ty * ground_ty * nat)%type.
+
+Obligation Tactic := program_simpl ; intuition ;
+     repeat 
+       (match goal with
+          | [H : ex _ |- _] => let v := fresh "v" in destruct H as [v H]
+          | [H : False |- _] => elim H
+          | [H : _ \/ _ |- _] => destruct H
+          | [H : _ = _ |- _] => inverts* H
+        end).
+
+Program Fixpoint lookup_gen_list (t t' : ground_ty) (l : gen_list) : 
+  {n | In (t,t',n) l} + {~ exists n, In (t,t',n) l} :=
+  match l with
+    | nil => inright _ _
+    | x :: l' => 
+        match x with
+          | (a,b,c) => 
+              match eq_ground_ty_dec t a, eq_ground_ty_dec b t' with
+                | left _, left _ => inleft _ (exist _ c _)
+                | right _, left _ => 
+                    match lookup_gen_list t t' l' with
+                      | inleft x => inleft _ x
+                      | inright _ => inright _ _
+                    end
+                | left _, right _ => 
+                    match lookup_gen_list t t' l' with
+                      | inleft x => inleft _ x
+                      | inright _ => inright _ _
+                    end
+                | right _, right _ => 
+                    match lookup_gen_list t t' l' with
+                      | inleft x => inleft _ x
+                      | inright _ => inright _ _
+                    end
+              end
+        end
+  end.
+
+Definition lgen_ground (t t' t1 : ground_ty) :=
+  leq_ground t1 t /\ leq_ground t1 t' /\ forall u, leq_ground u t /\ leq_ground u t' -> leq_ground u t1.
+
+Definition lgen_state := (ground_ty * (gen_list * nat)%type)%type.
+
+Obligation Tactic := 
+           unfold lgen_ground in * ; program_simpl ; intuition ; 
+               repeat (match goal with 
+                        | [H : leq_ground _ _ |- _] => inverts* H
+                        | [H : ?n = ?n -> False |- _] => elim H ; auto
+                       end).
+
+Program Fixpoint lgen_ground_aux (t t' : ground_ty) (l : gen_list) (m : nat) : {p | lgen_ground t t' (@fst ground_ty (gen_list * nat) p)} :=
+  match t,t' with
+    | skolem n, skolem n' =>
+        match eq_nat_dec n n' with
+          | left _  => exist _ (skolem n, (l, m)) _
+          | right _ => 
+              match lookup_gen_list (skolem n) (skolem n') l with 
+                | inleft (exist x _) => exist _ (skolem x, (l,m)) _
+                | inright _ => exist _ (skolem m, ((skolem n, skolem n',m) :: l, S m)) _
+              end
+        end
+    | skolem n, con n' =>
+        match lookup_gen_list (skolem n) (con n') l with
+          | inleft (exist x _) => exist _ (skolem x, (l,m)) _
+          | inright _ => exist _ (skolem m, ((skolem n, con n',m) :: l, S m)) _
+        end
+    | skolem n, app f r =>
+        match lookup_gen_list (skolem n) (app f r) l with
+          | inleft (exist x _) => exist _ (skolem x, (l,m)) _
+          | inright _ => exist _ (skolem m, ((skolem n,app f r,m) :: l, S m)) _            
+        end
+    | con n, con n' => 
+        match eq_nat_dec n n' with
+          | left _ => exist _ (con n, (l,m)) _
+          | right _ => 
+              match lookup_gen_list (con n) (con n') l with
+                | inleft (exist x _) => exist _ (skolem x, (l,m)) _
+                | inright _ => exist _ (skolem m, ((con n,con n',m) :: l, S m)) _
+              end
+        end
+    | con n, skolem n' =>
+        match lookup_gen_list (con n) (skolem n') l with
+          | inleft (exist x _) => exist _ (skolem x, (l,m)) _
+          | inright _ => exist _ (skolem m, ((con n, skolem n',m) :: l, S m)) _
+        end  
+    | con n, app f r =>
+        match lookup_gen_list (con n) (app f r) l with
+          | inleft (exist x _) => exist _ (skolem x, (l,m)) _
+          | inright _ => exist _ (skolem m, ((con n, app f r,m) :: l, S m)) _
+        end    
+    | app f r, con n =>
+        match lookup_gen_list (app f r) (con n) l with
+          | inleft (exist x _) => exist _ (skolem x, (l,m)) _
+          | inright _ => exist _ (skolem m, ((app f r, con n,m) :: l, S m)) _
+        end  
+    | app f r, skolem n =>
+        match lookup_gen_list (app f r) (skolem n) l with
+          | inleft (exist x _) => exist _ (skolem x, (l,m)) _
+          | inright _ => exist _ (skolem m, ((app f r, skolem n,m) :: l, S m)) _
+        end    
+    | app f r, app f' r' =>
+        match lgen_ground_aux f f' l m with
+          | (t,(l',m')) => 
+              match lgen_ground_aux r r' l' m' with
+                | (t', (l'', m'')) => 
+                    exist _ (app t t', (l'', m'')) _
+              end
+        end 
+  end.
